RocqOfRust/revm/revm_interpreter/links/interpreter.v
@@ -80,7 +80,6 @@ Module Impl_Interpreter.
     Proof.
     constructor.
     run_symbolic.
-    eapply (@run_halt IW H IW_types H0 run_InterpreterTypes_for_IW).
   Defined.
 
   Global Opaque run_halt_underflow.
@@ -98,7 +97,6 @@ Module Impl_Interpreter.
   Proof.
     constructor.
     run_symbolic.
-    eapply (@run_halt IW H IW_types H0 run_InterpreterTypes_for_IW).
   Defined.
   Global Opaque run_halt_overflow.
 
@@ -115,7 +113,6 @@ Module Impl_Interpreter.
   Proof.
     constructor.
     run_symbolic.
-    eapply (@run_halt IW H IW_types H0 run_InterpreterTypes_for_IW).
   Defined.
   Global Opaque run_halt_memory_oog.
 
